src/pipes/tactic.lean
@@ -1,0 +1,23 @@
+
+namespace tactic
+open lean.parser interactive interactive.types
+open tactic.interactive (generalize cases_arg_p)
+local postfix `?`:9000 := optional
+local postfix `*`:9000 := many
+
+lemma cast_eq_of_heq {α β} {x : α} {y : β}
+  (h : α = β)
+  (h' : cast h x = y)
+: x == y :=
+by { subst β, subst y, symmetry, simp [cast_heq] }
+
+meta def elim_cast (e : parse texpr) (n : parse (tk "with" *> ident)) : tactic unit :=
+do let h : name := ("H" ++ n.to_string : string),
+   interactive.generalize h () (``(cast _ %%e), n),
+   asm ← get_local h,
+   to_expr ``(cast_eq_of_heq _ %%asm) >>= note h none,
+   clear asm
+
+run_cmd add_interactive [`elim_cast]
+
+end tactic
